Backport improvements to proof

src/program_proof/simplepb/apps/closed_wpcs.v
@@ -1,5 +1,6 @@
 From Perennial.program_proof Require Import grove_prelude.
 From Goose.github_com.mit_pdos.gokv.simplepb.apps Require Import closed.
+From iris.base_logic Require Import ghost_map.
 
 From Perennial.goose_lang Require adequacy dist_adequacy.
 From Perennial.goose_lang.ffi Require grove_ffi_adequacy.
@@ -8,33 +9,32 @@ From Perennial.program_logic Require dist_lang.
 From Perennial.program_proof.bank Require Export bank_proof.
 From Perennial.program_proof.lock Require Export lock_proof.
 From Perennial.program_proof.simplepb Require Import pb_init_proof pb_definitions.
-From Perennial.program_proof.simplepb Require Import kv_proof.
+From Perennial.program_proof.simplepb Require Import kv_proof config_proof.
 From Perennial.program_proof.simplepb.simplelog Require Import proof.
 From Perennial.program_proof.simplepb.apps Require Import clerkpool_proof.
 From Perennial.program_proof.grove_shared Require Import urpc_proof.
 From Perennial.goose_lang Require Import crash_borrow crash_modality.
+From Perennial.goose_lang Require Import recovery_lifting.
 
 Section closed_wpcs.
 
 Context `{!heapGS Σ}.
 Context `{!ekvG Σ}.
-
-Lemma wpc_kv_replica_main γsys γsrv Φc fname me configHost :
-  ((∃ data' : list u8, fname f↦data' ∗ ▷ file_crash (own_Server_ghost_f γsys γsrv) data') -∗
+Context {kvParams:ekvParams.t}.
+Lemma wpc_kv_replica_main γ γsrv Φc fname me configHost data :
+  ((∃ data' : list u8, fname f↦data' ∗ ▷ kv_crash_resources γ γsrv data') -∗
     Φc) -∗
-  config_protocol_proof.is_pb_config_host configHost γsys -∗
-  is_pb_host me γsys γsrv -∗
-  is_pb_system_invs γsys -∗
-  (∃ data : list u8, fname f↦data ∗ file_crash (own_Server_ghost_f γsys γsrv) data) -∗
+  ("#Hconf" ∷ is_kv_config_host configHost γ ∗
+   "#Hhost" ∷ is_kv_replica_host me γ γsrv ∗
+   "Hfile" ∷ fname f↦ data ∗
+   "Hcrash" ∷ kv_crash_resources γ γsrv data
+  ) -∗
   WPC kv_replica_main #(LitString fname) #me #configHost @ ⊤
   {{ _, True }}
   {{ Φc }}
 .
 Proof.
-  (* TODO: all the invs *)
-  iIntros "HΦc #HconfHost #Hpbhost #Hinvs Hpre".
-  iNamed "Hinvs".
-  iDestruct "Hpre" as (?) "[Hfile Hcrash]".
+  iIntros "HΦc H". iNamed "H".
 
   unfold kv_replica_main.
   wpc_call.
@@ -63,7 +63,7 @@ Proof.
   { iAccu. }
   {
     iModIntro.
-    instantiate (1:=(|C={⊤}=> ∃ data', fname f↦ data' ∗ ▷ file_crash (own_Server_ghost_f γsys γsrv) data')).
+    instantiate (1:=(|C={⊤}=> ∃ data', fname f↦ data' ∗ ▷ kv_crash_resources γ γsrv data')).
     iIntros "[H1 H2]".
     iModIntro.
     iExists _.
@@ -79,11 +79,8 @@ Proof.
     done. }
   iApply wp_wpc.
   wp_pures.
-
-  wp_apply (wp_Start with "[Hfile_ctx]").
-  {
-    iFrame "∗#".
-  }
+  wp_apply (wp_Start with "[$Hfile_ctx]").
+  { iFrame "#". }
   wp_pures.
   done.
 Qed.
@@ -97,12 +94,103 @@ Definition lconfigHost : u64 := (U64 110).
 Definition lr1Host: u64 := (U64 101).
 Definition lr2Host: u64 := (U64 102).
 
+Lemma wp_dconfig_main γconf :
+  "HconfInit" ∷ makeConfigServer_pre γconf [dr1Host; dr2Host] ∗
+  "#Hhost" ∷ is_config_host dconfigHost γconf -∗
+  WP dconfig_main #() {{ _, True }}
+.
+Proof.
+  iNamed 1.
+  wp_call.
+  wp_apply (wp_NewSlice).
+  iIntros (?) "Hsl".
+  wp_apply wp_ref_to.
+  { done. }
+  iIntros (servers_ptr) "Hservers".
+  wp_pures.
+
+  wp_apply (wp_LoadAt with "[$Hservers]").
+  iIntros "Hservers".
+  wp_apply (wp_SliceAppend with "Hsl").
+  iIntros (?) "Hsl".
+  wp_apply (wp_StoreAt with "[$Hservers]").
+  { done. }
+  iIntros "Hservers".
+
+  wp_apply (wp_LoadAt with "[$Hservers]").
+  iIntros "Hservers".
+  wp_apply (wp_SliceAppend with "Hsl").
+  iIntros (?) "Hsl".
+  wp_apply (wp_StoreAt with "[$Hservers]").
+  { done. }
+  iIntros "Hservers".
+
+  wp_apply (wp_LoadAt with "[$Hservers]").
+  iIntros "Hservers".
+  iDestruct (own_slice_to_small with "Hsl") as "Hsl".
+  rewrite replicate_0.
+  simpl.
+  wp_apply (config_proof.wp_MakeServer with "[$HconfInit $Hsl]").
+  iIntros (?) "#Hissrv".
+  wp_apply (wp_Server__Serve with "[$]").
+  {
+    iFrame "Hissrv".
+  }
+  wp_pures.
+  done.
+Qed.
+
+Lemma wp_lconfig_main γconf :
+  "HconfInit" ∷ makeConfigServer_pre γconf [lr1Host; lr2Host] ∗
+  "#Hhost" ∷ is_config_host lconfigHost γconf -∗
+  WP lconfig_main #() {{ _, True }}
+.
+Proof.
+  iNamed 1.
+  wp_call.
+  wp_apply (wp_NewSlice).
+  iIntros (?) "Hsl".
+  wp_apply wp_ref_to.
+  { done. }
+  iIntros (servers_ptr) "Hservers".
+  wp_pures.
+
+  wp_apply (wp_LoadAt with "[$Hservers]").
+  iIntros "Hservers".
+  wp_apply (wp_SliceAppend with "Hsl").
+  iIntros (?) "Hsl".
+  wp_apply (wp_StoreAt with "[$Hservers]").
+  { done. }
+  iIntros "Hservers".
+
+  wp_apply (wp_LoadAt with "[$Hservers]").
+  iIntros "Hservers".
+  wp_apply (wp_SliceAppend with "Hsl").
+  iIntros (?) "Hsl".
+  wp_apply (wp_StoreAt with "[$Hservers]").
+  { done. }
+  iIntros "Hservers".
+
+  wp_apply (wp_LoadAt with "[$Hservers]").
+  iIntros "Hservers".
+  iDestruct (own_slice_to_small with "Hsl") as "Hsl".
+  rewrite replicate_0.
+  simpl.
+  wp_apply (config_proof.wp_MakeServer with "[$HconfInit $Hsl]").
+  iIntros (?) "#Hissrv".
+  wp_apply (wp_Server__Serve with "[$]").
+  {
+    iFrame "Hissrv".
+  }
+  wp_pures.
+  done.
+Qed.
 
 Context `{!bankG Σ}.
-Lemma wp_makeBankClerk γlk γkv :
+Lemma wp_makeBankClerk γlk γkv (kvParams1 kvParams2:ekvParams.t):
   {{{
-        "#Hhost1" ∷ is_kv_config dconfigHost γkv ∗
-        "#Hhost2" ∷ is_kv_config lconfigHost γlk ∗
+        "#Hhost1" ∷ is_kv_config_host (params:=kvParams1) dconfigHost γkv ∗
+        "#Hhost2" ∷ is_kv_config_host (params:=kvParams2) lconfigHost γlk ∗
         "#Hbank" ∷ is_bank "init" (Build_lock_names (kv_ptsto γlk)) (kv_ptsto γkv) {[ "a1"; "a2" ]}
   }}}
     makeBankClerk #()
@@ -111,12 +199,14 @@ Lemma wp_makeBankClerk γlk γkv :
   }}}
 .
 Proof.
+  clear kvParams.
   iIntros (?) "Hpre HΦ".
   iNamed "Hpre".
   wp_lam.
-  wp_apply (wp_MakeKv with "[$Hhost1]").
+  wp_apply (wp_MakeKv (params:=kvParams1) with "[$Hhost1]").
   iIntros (?) "#Hkv".
   wp_pures.
+
   wp_apply (wp_MakeKv with "[$Hhost2]").
   iIntros (?) "Hlock_kv".
   wp_apply (wp_MakeLockClerk lockN with "[Hlock_kv]").
@@ -134,9 +224,9 @@ Proof.
 Qed.
 
 Definition bank_pre : iProp Σ :=
-  ∃ γkv γlk,
-  "#Hhost1" ∷ is_kv_config dconfigHost γkv ∗
-  "#Hhost2" ∷ is_kv_config lconfigHost γlk ∗
+  ∃ γkv γlk (p1 p2:ekvParams.t),
+  "#Hhost1" ∷ is_kv_config_host (params:=p1) dconfigHost γkv ∗
+  "#Hhost2" ∷ is_kv_config_host (params:=p2) lconfigHost γlk ∗
   "#Hbank" ∷ is_bank "init" (Build_lock_names (kv_ptsto γlk)) (kv_ptsto γkv) {[ "a1"; "a2" ]}
 .
 
@@ -153,7 +243,14 @@ Proof.
   iIntros (?) "Hpre HΦ".
   iNamed "Hpre".
   wp_lam.
-  wp_apply (wp_makeBankClerk with "[$]").
+  wp_apply (wp_makeBankClerk with "[]").
+  { (* FIXME: there are two parameter typeclass instances in context *)
+    clear kvParams.
+    iFrame "Hbank".
+    iSplit.
+    { iExact "Hhost1". }
+    { iExact "Hhost2". }
+  }
   iIntros (?) "Hck".
   wp_pures.
   wp_forBreak.
@@ -177,7 +274,14 @@ Proof.
   iIntros (?) "Hpre HΦ".
   iNamed "Hpre".
   wp_lam.
-  wp_apply (wp_makeBankClerk with "[$]").
+  wp_apply (wp_makeBankClerk with "[]").
+  { (* FIXME: there are two parameter typeclass instances in context *)
+    clear kvParams.
+    iFrame "Hbank".
+    iSplit.
+    { iExact "Hhost1". }
+    { iExact "Hhost2". }
+  }
   iIntros (?) "Hck".
   wp_pures.
   wp_forBreak.
@@ -189,3 +293,231 @@ Proof.
 Qed.
 
 End closed_wpcs.
+
+Section closed_wprs.
+
+Context {kvParams:ekvParams.t}.
+
+#[global]
+Instance is_kv_config_into_crash `{hG0: !heapGS Σ} `{!ekvG Σ} u γ:
+  IntoCrash (is_kv_config_host u γ)
+    (λ hG, ⌜ hG0.(goose_globalGS) = hG.(goose_globalGS) ⌝ ∗ is_kv_config_host u γ)%I
+.
+Proof.
+  rewrite /IntoCrash /is_kv_config_host.
+  iIntros "$". iIntros; eauto.
+Qed.
+
+#[global]
+Instance is_kv_replica_host_into_crash `{hG0: !heapGS Σ} `{!ekvG Σ} u γ γsrv:
+  IntoCrash (is_kv_replica_host u γ γsrv)
+    (λ hG, ⌜ hG0.(goose_globalGS) = hG.(goose_globalGS) ⌝ ∗ is_kv_replica_host u γ γsrv)%I
+.
+Proof.
+  rewrite /IntoCrash /is_kv_replica_host.
+  iIntros "$". iIntros; eauto.
+Qed.
+
+#[global]
+Instance kv_crash_into_crash `{hG0: !heapGS Σ} `{!ekvG Σ} a b c:
+  IntoCrash (kv_crash_resources a b c)
+    (λ hG, (kv_crash_resources a b c))%I.
+Proof.
+  rewrite /IntoCrash /file_crash.
+  iIntros "$". iIntros; eauto.
+Qed.
+
+Local Definition crash_cond {Σ} `{ekvG Σ} {fname γ γsrv} :=
+  (λ hG : heapGS Σ, ∃ data, fname f↦ data ∗ ▷ kv_crash_resources γ γsrv data)%I.
+
+Lemma wpr_kv_replica_main fname me configHost γ γsrv {Σ} `{HKV: ekvG Σ}
+                               {HG} {HL}:
+  let hG := {| goose_globalGS := HG; goose_localGS := HL |} in
+  ("#Hconf" ∷ is_kv_config_host configHost γ ∗
+   "#Hhost" ∷ is_kv_replica_host me γ γsrv ∗
+   "Hcrash" ∷ kv_crash_resources γ γsrv [] ∗
+   "Hfile" ∷ fname f↦ []
+  ) -∗
+  wpr NotStuck ⊤ (kv_replica_main #(LitString fname) #me #configHost) (kv_replica_main #(LitString fname) #me #configHost) (λ _ : goose_lang.val, True)
+    (λ _ , True) (λ _ _, True).
+Proof.
+  intros.
+  iNamed 1.
+  iApply (idempotence_wpr with "[Hfile Hcrash] []").
+  {
+    instantiate (1:=crash_cond).
+    simpl.
+    wpc_apply (wpc_kv_replica_main with "[]").
+    { iIntros "$". }
+    iFrame "∗#".
+  }
+  { (* recovery *)
+    rewrite /hG.
+    clear hG.
+    iModIntro.
+    iIntros (????) "Hcrash".
+    iNext.
+    iDestruct "Hcrash" as (?) "[Hfile Hcrash]".
+    simpl.
+    set (hG' := HeapGS _ _ hL').
+    iDestruct "Hconf" as "-#Hconf".
+    iDestruct "Hhost" as "-#Hhost".
+    iCrash.
+    iIntros "_".
+    destruct hL as [HG'' ?].
+    iSplit; first done.
+    iDestruct "Hconf" as "(%&Hconf)".
+    iDestruct "Hhost" as "(%&Hhost)".
+    subst.
+    simpl in *.
+    clear hG'.
+    clear hL'.
+    (* overcome impedence mismatch between heapGS (bundled) and gooseGLobalGS+gooseLocalGS (split) proofs *)
+    set (hG2' := HeapGS _ _ goose_localGS).
+    simpl.
+    wpc_apply (wpc_kv_replica_main (heapGS0:=hG2') with "[]").
+    { iIntros "H".
+      iDestruct "H" as (?) "[Hfile Hcrash]".
+      iExists _.
+      iFrame.
+    }
+    iFrame "∗#".
+  }
+Qed.
+
+Lemma wpr_dconfig_main {Σ} `{HKV: ekvG Σ} γ
+                               {HG} {HL}:
+  let hG := {| goose_globalGS := HG; goose_localGS := HL |} in
+  ("#Hhost" ∷ is_config_host dconfigHost γ ∗
+   "Hcrash" ∷ makeConfigServer_pre γ [dr1Host ; dr2Host]
+  ) -∗
+  wpr NotStuck ⊤ (dconfig_main #())
+      (#()) (λ _ : goose_lang.val, True)
+    (λ _ , True) (λ _ _, True).
+Proof.
+  intros.
+  iNamed 1.
+  iApply (idempotence_wpr with "[-] []").
+  {
+    instantiate (1:=(λ _, True)%I).
+    simpl.
+    iApply wp_wpc.
+    wp_apply (wp_dconfig_main with "[$]").
+  }
+  { (* recovery *)
+    rewrite /hG.
+    clear hG.
+    iModIntro.
+    iIntros (????) "Hcrash".
+    iNext.
+    set (hG' := HeapGS _ _ hL').
+    iDestruct "Hhost" as "-#Hhost".
+    iCrash.
+    iIntros "_".
+    iSplit; first done.
+    by wpc_pures.
+  }
+Qed.
+
+Lemma wpr_lconfig_main {Σ} `{HKV: ekvG Σ} γ
+                               {HG} {HL}:
+  let hG := {| goose_globalGS := HG; goose_localGS := HL |} in
+  ("#Hhost" ∷ is_config_host lconfigHost γ ∗
+   "Hcrash" ∷ makeConfigServer_pre γ [lr1Host ; lr2Host]
+  ) -∗
+  wpr NotStuck ⊤ (lconfig_main #())
+      (#()) (λ _ : goose_lang.val, True)
+    (λ _ , True) (λ _ _, True).
+Proof.
+  intros.
+  iNamed 1.
+  iApply (idempotence_wpr with "[-] []").
+  {
+    instantiate (1:=(λ _, True)%I).
+    simpl.
+    iApply wp_wpc.
+    wp_apply (wp_lconfig_main with "[$]").
+  }
+  { (* recovery *)
+    rewrite /hG.
+    clear hG.
+    iModIntro.
+    iIntros (????) "Hcrash".
+    iNext.
+    set (hG' := HeapGS _ _ hL').
+    iDestruct "Hhost" as "-#Hhost".
+    iCrash.
+    iIntros "_".
+    iSplit; first done.
+    by wpc_pures.
+  }
+Qed.
+
+End closed_wprs.
+
+Section closed_init.
+
+Context `{!gooseGlobalGS Σ}.
+
+Existing Instance toEsmParams1.
+Lemma alloc_vkv (params:ekvParams.t) configHost allocated `{!ekvG Σ}:
+  length ekvParams.initconfig > 0 →
+  configHost c↦ ∅ ∗
+  ([∗ list] h ∈ ekvParams.initconfig, h c↦ ∅)
+  ={⊤}=∗ (∃ γ,
+
+  (* system-wide: allows clients to connect to the system, and gives them ownership of keys *)
+  ([∗ set] k ∈ allocated, kv_ptsto γ k "") ∗
+  is_kv_config_host configHost γ ∗
+
+  (* for each kv replica server:  *)
+  ([∗ list] host ∈ ekvParams.initconfig,
+     ∃ γsrv,
+     is_kv_replica_host host γ γsrv ∗
+     kv_crash_resources γ γsrv []
+  )) ∗
+
+  (* for each the config server:  *)
+  (∃ γconf,
+    is_config_host configHost γconf ∗
+    makeConfigServer_pre γconf ekvParams.initconfig
+  )
+.
+Proof.
+  intros.
+  iIntros "[HconfChan Hchan]".
+  iMod (alloc_simplepb_system with "[$Hchan] [$HconfChan]") as (?) "H"; try done.
+  iDestruct "H" as "(Hlog & #Hhosts & Hsrvs & HconfSrvs)".
+  iFrame "HconfSrvs".
+  iMod (ghost_map_alloc (gset_to_gmap "" allocated)) as (γkv_gn) "[Hauth Hkvs]".
+  iExists (Build_kv_names _ _).
+  rewrite big_sepM_gset_to_gmap.
+  iFrame "Hkvs".
+  iAssert (|={⊤}=> is_kv_config_host configHost _)%I with "[Hlog Hauth]" as ">#Hhosts2".
+  {
+    rewrite /is_kv_config_host.
+    iMod (esm_proof.alloc_esm with "Hlog") as (??) "(#He1 & #He2 & Hlog)".
+    repeat iExists _.
+    instantiate (1:=Build_kv_names _ _). simpl.
+    iFrame "#".
+    iMod (inv_alloc with "[-]"); last done.
+    iNext. repeat iExists _.
+    iFrame. rewrite /own_kvs /=.
+    iExists _; iFrame.
+    iExactEq "Hauth".
+    repeat f_equal.
+    rewrite /kv_vsm_proof.compute_state /=.
+    rewrite map_empty_union. done.
+  }
+  iModIntro.
+  iFrame "#".
+  simpl. rewrite app_nil_r.
+  iApply (big_sepL_impl with "Hsrvs []").
+  iIntros "!# * %Hlookup H".
+  iDestruct "H" as (?) "[#HpbHost Hghost]".
+  iExists _. rewrite /is_kv_replica_host. iFrame "HpbHost".
+  rewrite /kv_crash_resources.
+  iLeft. iFrame. done.
+Qed.
+
+End closed_init.
