src/program_proof/simplepb/apps/closed_proof.v
@@ -30,47 +30,14 @@ Definition grove_dist_adequate
 
 Definition kv_pbΣ := #[heapΣ; ekvΣ; bankΣ].
 
-#[global]
-Instance sys_inv_into_crash `{!heapGS Σ} EntryType `{!pbG Σ} γsys :
-  IntoCrash (is_pb_system_invs γsys) (λ hG', @is_pb_system_invs EntryType Σ (_ hG') _ γsys)
-.
-Proof.
-  rewrite /IntoCrash /is_pb_system_invs.
-  iIntros "$". iIntros; eauto.
-Qed.
+(* There's one of these in kvee_proof.v, so I got rid of this.
+   This is probably a remnant of an older version of the proof in which the subG
+   wasn't proven anywhere else.
+ *)
+Local Instance subG_ekvΣ {Σ} : subG kv_pbΣ Σ → ekvG Σ.
+Proof. intros. solve_inG. Qed.
 
-(* The globalGS equality should actually always be the case (or more precisely,
- we should be unbundling, but let's include it here in the conclusion as a
- hack *)
-#[global]
-Instance is_pb_host_into_crash `{hG0: !heapGS Σ} PBRecord `{!pbG Σ} u γ1 γ2 :
-  IntoCrash (is_pb_host u γ1 γ2)
-    (λ hG, ⌜ hG0.(goose_globalGS) = hG.(goose_globalGS) ⌝ ∗ is_pb_host (pb_record:=PBRecord) u γ1 γ2)%I
-.
-Proof.
-  rewrite /IntoCrash /is_pb_host.
-  iIntros "$". iIntros; eauto.
-Qed.
-
-#[global]
-Instance is_pb_config_host_into_crash `{hG0: !heapGS Σ} PBRecord `{!pbG Σ} u γ:
-  IntoCrash (is_pb_config_host u γ)
-    (λ hG, ⌜ hG0.(goose_globalGS) = hG.(goose_globalGS) ⌝ ∗ is_pb_config_host (pb_record:=PBRecord) u γ)%I
-.
-Proof.
-  rewrite /IntoCrash /is_pb_host.
-  iIntros "$". iIntros; eauto.
-Qed.
-
-#[global]
-Instance is_kv_config_into_crash `{hG0: !heapGS Σ} `{!ekvG Σ} u γ:
-  IntoCrash (is_kv_config u γ)
-    (λ hG, ⌜ hG0.(goose_globalGS) = hG.(goose_globalGS) ⌝ ∗ is_kv_config u γ)%I
-.
-Proof.
-  rewrite /IntoCrash /is_kv_config.
-  iIntros "$". iIntros; eauto.
-Qed.
+Definition replica_fname := "kv.data".
 
 #[global]
 Instance is_bank_into_crash `{hG0: !heapGS Σ} `{!bankG Σ} a b c d :
@@ -81,178 +48,6 @@ Proof.
   rewrite /IntoCrash /is_bank.
   iIntros "$". iIntros; eauto.
 Qed.
-
-#[global]
-Instance file_crash_into_crash `{hG0: !heapGS Σ} SMRecord `{!pbG Σ} γsys γsrv1 data:
-  IntoCrash (file_crash (own_Server_ghost_f γsys γsrv1) data)
-    (λ hG, (file_crash (sm_record := SMRecord) (own_Server_ghost_f γsys γsrv1 ) data)).
-Proof.
-  rewrite /IntoCrash /file_crash.
-  iIntros "$". iIntros; eauto.
-Qed.
-
-Definition kv_replica_main_crash_cond `{ekvG Σ} γsys fname γsrv1:=
-(λ hG : heapGS Σ, ∃ data',
-    (fname f↦ data') ∗ ▷ file_crash (own_Server_ghost_f γsys γsrv1) data')%I.
-
-Lemma wpr_kv_replica_main fname me configHost γsys γsrv {Σ} {HKV: ekvG Σ}
-                               {HG} {HL}:
-  let hG := {| goose_globalGS := HG; goose_localGS := HL |} in
-  "Hinvs" ∷ is_pb_system_invs γsys -∗
-  "Hsrvhost1" ∷ is_pb_host me γsys γsrv -∗
-  "Hconfhost" ∷ is_pb_config_host configHost γsys -∗
-  "Hinit" ∷ fname f↦[] -∗
-  "Hfile_crash" ∷ file_crash (own_Server_ghost_f γsys γsrv) [] -∗
-  wpr NotStuck ⊤ (kv_replica_main #(LitString fname) #me #configHost) (kv_replica_main #(LitString fname) #me #configHost) (λ _ : goose_lang.val, True)
-    (λ _ , True) (λ _ _, True).
-Proof.
-   iIntros. iNamed.
-   iApply (idempotence_wpr with "[Hinit Hfile_crash] []").
-   {
-     instantiate (1:=kv_replica_main_crash_cond γsys fname γsrv).
-     simpl.
-     wpc_apply (wpc_kv_replica_main γsys γsrv with "[] [$] [$] [$]").
-     { iIntros "$". }
-     iExists _. iFrame.
-   }
-   { (* recovery *)
-     rewrite /hG.
-     clear hG.
-     iModIntro.
-     iIntros (????) "Hcrash".
-     iNext.
-     iDestruct "Hcrash" as (?) "[Hfile Hcrash]".
-     simpl.
-     set (hG' := HeapGS _ _ hL').
-     iDestruct "Hinvs" as "-#Hinvs".
-     iDestruct "Hsrvhost1" as "-#Hsrvhost1".
-     iDestruct "Hconfhost" as "-#Hconfhost".
-     iCrash.
-     iIntros "_".
-     destruct hL as [HG'' ?].
-     iSplit; first done.
-     iDestruct "Hsrvhost1" as "(%&Hsrvhost1)".
-     iDestruct "Hconfhost" as "(%&Hconfhost)".
-     subst.
-     clear hG'.
-     clear hL'.
-     (* overcome impedence mismatch between heapGS (bundled) and gooseGLobalGS+gooseLocalGS (split) proofs *)
-     set (hG2' := HeapGS _ _ goose_localGS).
-     simpl.
-     wpc_apply (wpc_kv_replica_main (heapGS0:=hG2') γsys γsrv with "[] [$] [$] [$]").
-     { iIntros "H".
-       iDestruct "H" as (?) "[Hfile Hcrash]".
-       iExists _.
-       iFrame.
-     }
-     iExists _. iFrame.
-   }
-Qed.
-
-Lemma wp_lconfig_main γconf {Σ} {HKV: ekvG Σ} {HG} {HL}:
-  let hG := {| goose_globalGS := HG; goose_localGS := HL |} in
-  "HconfInit" ∷ makeConfigServer_pre γconf [lr1Host; lr2Host] ∗
-  "#Hhost" ∷ is_config_host lconfigHost γconf -∗
-  WP lconfig_main #() {{ _, True }}
-.
-Proof.
-  intros ?.
-  iNamed 1.
-  wp_call.
-  wp_apply (wp_NewSlice).
-  iIntros (?) "Hsl".
-  wp_apply wp_ref_to.
-  { done. }
-  iIntros (servers_ptr) "Hservers".
-  wp_pures.
-
-  wp_apply (wp_LoadAt with "[$Hservers]").
-  iIntros "Hservers".
-  wp_apply (wp_SliceAppend with "Hsl").
-  iIntros (?) "Hsl".
-  wp_apply (wp_StoreAt with "[$Hservers]").
-  { done. }
-  iIntros "Hservers".
-
-  wp_apply (wp_LoadAt with "[$Hservers]").
-  iIntros "Hservers".
-  wp_apply (wp_SliceAppend with "Hsl").
-  iIntros (?) "Hsl".
-  wp_apply (wp_StoreAt with "[$Hservers]").
-  { done. }
-  iIntros "Hservers".
-
-  wp_apply (wp_LoadAt with "[$Hservers]").
-  iIntros "Hservers".
-  iDestruct (own_slice_to_small with "Hsl") as "Hsl".
-  rewrite replicate_0.
-  simpl.
-  wp_apply (config_proof.wp_MakeServer with "[$HconfInit $Hsl]").
-  iIntros (?) "#Hissrv".
-  wp_apply (wp_Server__Serve with "[$]").
-  {
-    iFrame "Hissrv".
-  }
-  wp_pures.
-  done.
-Qed.
-
-Lemma wp_dconfig_main γconf {Σ} {HKV: ekvG Σ} {HG} {HL}:
-  let hG := {| goose_globalGS := HG; goose_localGS := HL |} in
-  "HconfInit" ∷ makeConfigServer_pre γconf [dr1Host; dr2Host] ∗
-  "#Hhost" ∷ is_config_host dconfigHost γconf -∗
-  WP dconfig_main #() {{ _, True }}
-.
-Proof.
-  intros ?.
-  iNamed 1.
-  wp_call.
-  wp_apply (wp_NewSlice).
-  iIntros (?) "Hsl".
-  wp_apply wp_ref_to.
-  { done. }
-  iIntros (servers_ptr) "Hservers".
-  wp_pures.
-
-  wp_apply (wp_LoadAt with "[$Hservers]").
-  iIntros "Hservers".
-  wp_apply (wp_SliceAppend with "Hsl").
-  iIntros (?) "Hsl".
-  wp_apply (wp_StoreAt with "[$Hservers]").
-  { done. }
-  iIntros "Hservers".
-
-  wp_apply (wp_LoadAt with "[$Hservers]").
-  iIntros "Hservers".
-  wp_apply (wp_SliceAppend with "Hsl").
-  iIntros (?) "Hsl".
-  wp_apply (wp_StoreAt with "[$Hservers]").
-  { done. }
-  iIntros "Hservers".
-
-  wp_apply (wp_LoadAt with "[$Hservers]").
-  iIntros "Hservers".
-  iDestruct (own_slice_to_small with "Hsl") as "Hsl".
-  rewrite replicate_0.
-  simpl.
-  wp_apply (config_proof.wp_MakeServer with "[$HconfInit $Hsl]").
-  iIntros (?) "#Hissrv".
-  wp_apply (wp_Server__Serve with "[$]").
-  {
-    iFrame "Hissrv".
-  }
-  wp_pures.
-  done.
-Qed.
-
-(* There's one of these in kvee_proof.v, so I got rid of this.
-   This is probably a remnant of an older version of the proof in which the subG
-   wasn't proven anywhere else.
- *)
-Local Instance subG_ekvΣ {Σ} : subG kv_pbΣ Σ → ekvG Σ.
-Proof. intros. solve_inG. Qed.
-
-Definition replica_fname := "kv.data".
 
 (* FIXME: put this in the file that defines ekvΣ? *)
 Opaque ekvΣ.
@@ -313,104 +108,58 @@ Proof.
   iSplitR ""; last first.
   { iModIntro. iMod (fupd_mask_subseteq ∅); eauto. }
 
-  (* SET UP RSM SYTEM *)
-  (* First, pre-set up the two pairs of KV replica servers *)
-  iMod (prealloc_simplepb_server) as (γsrvd1) "[#Hdsrv1wit Hdsrv1]".
-  iMod (prealloc_simplepb_server) as (γsrvd2) "[#Hdsrv2wit Hdsrv2]".
-  set (confdγs:=[γsrvd1 ; γsrvd2]).
-  iMod (alloc_simplepb_system confdγs with "[]") as (γdpb) "Hd".
-  { simpl. lia. }
-  { iIntros. rewrite /confdγs elem_of_list_In /= in H.
-    naive_solver. }
-
-  iDestruct "Hd" as "(#Hinvs & Hlog & #Hwits & Hconf1 & Hconf2 & #Hclient_invs)".
-
-  (* Now, set up the exactly-once kv system *)
-  iMod (alloc_ekv _ {[ "init"; "a1"; "a2" ]} with "Hlog") as (?) "[#Hclient_invs2 Hkvs]".
-
-  (* Now, set up all the hosts *)
-  iDestruct (big_sepM_delete with "Hchan") as "[HconfChan Hchan]".
-  { apply HdconfChan. } (* get out conf chan points-to for later *)
-
-  iDestruct (big_sepM_delete with "Hchan") as "[Hr1Chan Hchan]".
-  { rewrite lookup_delete_Some. split; last apply Hdr1Chan. done. }
-  iMod (pb_host_init dr1Host with "Hr1Chan") as "#Hsrvhost1".
-
-  iDestruct (big_sepM_delete with "Hchan") as "[Hr2Chan Hchan]".
-  { rewrite lookup_delete_Some.
-    rewrite lookup_delete_Some.
-    split; last (split ; last apply Hdr2Chan); done. }
-  iMod (pb_host_init dr2Host with "Hr2Chan") as "#Hsrvhost2".
-
-  set (dconf:=[dr1Host ; dr2Host]).
-  iMod (alloc_pb_config_ghost γdpb dconf confdγs with "[] Hconf1 Hconf2") as (γconf) "[#Hconf HconfInit]".
+  set (own_chans:=(λ l, [∗ list] h ∈ l, h c↦ ∅)%I).
+  iAssert (
+      own_chans [dr1Host ; dr2Host] ∗
+      own_chans [dconfigHost] ∗
+      own_chans [lr1Host ; lr2Host] ∗
+      own_chans [lconfigHost]
+    )%I with "[Hchan]" as "Hchans".
   {
-    iFrame "#".
-    by iApply big_sepL2_nil.
+    rewrite /own_chans.
+    repeat rewrite -big_sepL_app; simpl.
+    repeat (
+        iDestruct (big_sepM_delete with "Hchan") as "[$ Hchan]";
+        first (repeat rewrite lookup_delete_Some; try split_and!; try done)
+      ).
   }
+  iDestruct "Hchans" as "(Hd1 & Hd2 & Hl1 & Hl2)".
 
-  iMod (config_server_init dconfigHost γconf with "HconfChan") as "#Hconfhost".
-
-  iAssert (is_pb_config_host dconfigHost γdpb) with "[]" as "#HbConfHost".
-  { iExists _. iFrame "#". }
-  (* END SET UP RSM SYTEM *)
-  (* TODO: the above should probably be a lemma *)
-
-  (* SET UP RSM SYTEM *)
-  (* First, pre-set up the two pairs of KV replica servers *)
-  iMod (prealloc_simplepb_server) as (γsrvl1) "[#Hlsrv1wit Hlsrv1]".
-  iMod (prealloc_simplepb_server) as (γsrvl2) "[#Hlsrv2wit Hlsrv2]".
-  set (conflγs:=[γsrvl1 ; γsrvl2]).
-  iMod (alloc_simplepb_system conflγs with "[]") as (γlpb) "Hl".
-  { simpl. lia. }
-  { iIntros. rewrite /conflγs elem_of_list_In /= in H.
-    naive_solver. }
-
-  iDestruct "Hl" as "(#Hlinvs & Hllog & #Hlwits & Hlconf1 & Hlconf2 & #Hlclient_invs)".
-
-  (* Now, set up the exactly-once kv system *)
-  iMod (alloc_ekv _ {[ "init"; "a1"; "a2" ]} with "Hllog") as (?) "[#Hlclient_invs2 Hlkvs]".
-
-  (* Now, set up all the hosts *)
-  iDestruct (big_sepM_delete with "Hchan") as "[HlconfChan Hchan]".
-  { repeat rewrite lookup_delete_Some.
-    split_and!; last apply HlconfChan; done. }
-
-  iDestruct (big_sepM_delete with "Hchan") as "[Hlr1Chan Hchan]".
-  { repeat rewrite lookup_delete_Some. split_and!; last apply Hlr1Chan; done. }
-  iMod (pb_host_init lr1Host with "Hlr1Chan") as "#Hlsrvhost1".
-
-  iDestruct (big_sepM_delete with "Hchan") as "[Hlr2Chan Hchan]".
-  { repeat rewrite lookup_delete_Some.
-    split_and!; last apply Hlr2Chan; done. }
-  iMod (pb_host_init lr2Host with "Hlr2Chan") as "#Hlsrvhost2".
-
-  set (lconf:=[lr1Host ; lr2Host]).
-  iMod (alloc_pb_config_ghost γlpb lconf conflγs with "[] Hlconf1 Hlconf2") as (γlconf) "[#Hlconf HlconfInit]".
+  (* Allocate the kv system used for storing data *)
+  iMod (alloc_vkv (ekvParams.mk [dr1Host ; dr2Host ]) dconfigHost
+                  {[ "init"; "a1"; "a2" ]} with "[Hd1 Hd2]") as "[Hdkv Hdconf]"; try (simpl; lia).
   {
-    iFrame "#".
-    by iApply big_sepL2_nil.
+    rewrite /own_chans /=.
+    repeat iDestruct (wand_refl (_ ∗ _) with "[$]") as "[? ?]".
+    iFrame.
   }
+  iDestruct "Hdkv" as (γd)  "(Hkvs & #Hdhost & Hdsrvs)".
+  iSimpl in "Hdhost".
 
-  iMod (config_server_init lconfigHost γlconf with "HlconfChan") as "#Hlconfhost".
-
-  iAssert (is_pb_config_host lconfigHost γlpb) with "[]" as "#HlConfHost".
-  { iExists _. iFrame "#". }
-  (* END SET UP RSM SYTEM *)
+  (* Allocate the kv system used as a lockservice *)
+  iMod (alloc_vkv (ekvParams.mk [lr1Host ; lr2Host ]) lconfigHost
+                  {[ "init"; "a1"; "a2" ]} with "[Hl1 Hl2]") as "[Hlkv Hlconf]"; try (simpl; lia).
+  {
+    rewrite /own_chans /=.
+    repeat iDestruct (wand_refl (_ ∗ _) with "[$]") as "[? ?]".
+    iFrame.
+  }
+  iDestruct "Hlkv" as (γl)  "(Hlkvs & #Hlhost & Hlsrvs)".
+  iSimpl in "Hlhost".
 
   (* set up bank *)
   iAssert (|={⊤}=> is_bank "init" _ _ {[ "a1" ; "a2" ]})%I with "[Hlkvs Hkvs]" as ">#Hbank".
   {
     iDestruct (big_sepS_delete _ _ "init" with "Hlkvs") as "(Hinit&Hlkvs)".
     { set_solver. }
-    instantiate (2:=Build_lock_names (kv_ptsto γkv0)).
+    instantiate (2:=Build_lock_names (kv_ptsto γl)).
     rewrite /is_bank.
-    iMod (lock_alloc lockN {| kvptsto_lock := kv_ptsto γkv0 |} _ "init" with "[Hinit] [-]") as "$"; last done.
+    iMod (lock_alloc lockN {| kvptsto_lock := kv_ptsto γl |} _ "init" with "[Hinit] [-]") as "$"; last done.
     { iFrame. }
     iDestruct (big_sepS_delete _ _ "init" with "Hkvs") as "(Hinit&Hkvs)".
     { set_solver. }
     iLeft.
-    instantiate (1:=kv_ptsto γkv).
+    instantiate (1:=kv_ptsto γd).
     iFrame.
     iApply (big_sepS_sep).
     eassert (_ ∖ _ = {[ "a1"; "a2" ]}) as ->.
@@ -419,128 +168,75 @@ Proof.
   }
 
   iModIntro.
-  simpl. iSplitL "HconfInit".
+  simpl. iSplitL "Hdconf".
   {
     iIntros (HL) "Hfiles".
-    iModIntro.
     iExists (λ _, True%I), (λ _, True%I), (λ _ _, True%I).
-    set (hG' := HeapGS _ _ _). (* overcome impedence mismatch between heapGS (bundled) and gooseGLobalGS+gooseLocalGS (split) proofs *)
-    iApply (idempotence_wpr with "[HconfInit] []").
-    {
-      instantiate (1:=λ _, True%I).
-      simpl.
-      iApply wp_wpc.
-      iApply (wp_dconfig_main _ with "[$]").
-    }
-    { (* crash; there should actually be no crashes of the config server *)
-      iModIntro.
-      iIntros.
-      iModIntro.
-      rewrite /post_crash.
-      iIntros. iModIntro.
-      iSplit; first done. iIntros. iSplit; first done.
-      set (hG2' := HeapGS _ _ _). (* overcome impedence mismatch between heapGS (bundled) and gooseGLobalGS+gooseLocalGS (split) proofs *)
-      wpc_pures.
-      { done. }
-      done.
-    }
+    iModIntro.
+    set (hG' := HeapGS _ _ _).
+    iDestruct "Hdconf" as (?) "[#Hhost Hpre]".
+    iApply (wpr_dconfig_main with "[$]").
   }
-  iSplitL "HlconfInit".
+  simpl. iSplitL "Hlconf".
   {
     iIntros (HL) "Hfiles".
-    iModIntro.
     iExists (λ _, True%I), (λ _, True%I), (λ _ _, True%I).
-    set (hG' := HeapGS _ _ _). (* overcome impedence mismatch between heapGS (bundled) and gooseGLobalGS+gooseLocalGS (split) proofs *)
-    iApply (idempotence_wpr with "[HlconfInit] []").
-    {
-      instantiate (1:=λ _, True%I).
-      simpl.
-      iApply wp_wpc.
-      iApply (wp_lconfig_main _ with "[$]").
-    }
-    { (* crash; there should actually be no crashes of the config server *)
-      iModIntro.
-      iIntros.
-      iModIntro.
-      rewrite /post_crash.
-      iIntros. iModIntro.
-      iSplit; first done. iIntros. iSplit; first done.
-      set (hG2' := HeapGS _ _ _). (* overcome impedence mismatch between heapGS (bundled) and gooseGLobalGS+gooseLocalGS (split) proofs *)
-      wpc_pures.
-      { done. }
-      done.
-    }
+    iModIntro.
+    set (hG' := HeapGS _ _ _).
+    iDestruct "Hlconf" as (?) "[#Hhost Hpre]".
+    iApply (wpr_lconfig_main with "[$]").
   }
-  iSplitL "Hdsrv1".
+  iDestruct ("Hdsrvs") as "[Hdsrv Hdsrvs]".
+  iSplitL "Hdsrv".
   {
     iIntros (HL) "Hfiles".
     iDestruct (big_sepM_lookup_acc with "Hfiles") as "[HH _]".
     { done. }
-    iSpecialize ("Hdsrv1" $! γdpb with "[]").
-    { iApply "Hwits". iPureIntro. rewrite /confdγs elem_of_list_In /= //. naive_solver. }
     iModIntro.
     iExists (λ _, True%I), (λ _, True%I), (λ _ _, True%I).
     set (hG' := HeapGS _ _ _).
-    iAssert (file_crash (own_Server_ghost_f γdpb _) []) with "[Hdsrv1]" as "HfileCrash".
-    { iLeft. by iFrame. }
-    iApply (@wpr_kv_replica_main _ _ _ γdpb γsrvd1 with "[$] [$] [$] [$] [$]").
+    iDestruct "Hdsrv" as (?) "[H1 H2]".
+    iApply (wpr_kv_replica_main with "[- $H1]").
+    { iFrame "∗#". }
   }
-  (* TODO: do like above for replica main1 as separate lemma *)
-  iSplitL "Hdsrv2".
+  iDestruct ("Hdsrvs") as "[Hdsrv Hdsrvs]".
+  iSplitL "Hdsrv".
   {
     iIntros (HL) "Hfiles".
     iDestruct (big_sepM_lookup_acc with "Hfiles") as "[HH _]".
     { done. }
-    iSpecialize ("Hdsrv2" $! γdpb with "[]").
-    { iApply "Hwits". iPureIntro. rewrite /confdγs elem_of_list_In /= //. naive_solver. }
     iModIntro.
     iExists (λ _, True%I), (λ _, True%I), (λ _ _, True%I).
     set (hG' := HeapGS _ _ _).
-    iAssert (file_crash (own_Server_ghost_f γdpb _) []) with "[Hdsrv2]" as "HfileCrash".
-    { iLeft. by iFrame. }
-    iApply (@wpr_kv_replica_main _ _ _ γdpb γsrvd2 with "[$] [$] [$] [$] [$]").
+    iDestruct "Hdsrv" as (?) "[H1 H2]".
+    iApply (wpr_kv_replica_main with "[- $H1]").
+    { iFrame "∗#". }
   }
-  iSplitL "Hlsrv1".
+  iDestruct ("Hlsrvs") as "[Hlsrv Hlsrvs]".
+  iSplitL "Hlsrv".
   {
     iIntros (HL) "Hfiles".
     iDestruct (big_sepM_lookup_acc with "Hfiles") as "[HH _]".
     { done. }
-    iSpecialize ("Hlsrv1" $! γlpb with "[]").
-    { iApply "Hlwits". iPureIntro. rewrite /confdγs elem_of_list_In /= //. naive_solver. }
     iModIntro.
     iExists (λ _, True%I), (λ _, True%I), (λ _ _, True%I).
     set (hG' := HeapGS _ _ _).
-    iAssert (file_crash (own_Server_ghost_f γlpb _) []) with "[Hlsrv1]" as "HfileCrash".
-    { iLeft. by iFrame. }
-    iApply (@wpr_kv_replica_main _ _ _ γlpb γsrvl1 with "[$] [$] [$] [$] [$]").
+    iDestruct "Hlsrv" as (?) "[H1 H2]".
+    iApply (wpr_kv_replica_main with "[- $H1]").
+    { iFrame "∗#". }
   }
-  iSplitL "Hlsrv2".
+  iDestruct ("Hlsrvs") as "[Hlsrv Hlsrvs]".
+  iSplitL "Hlsrv".
   {
     iIntros (HL) "Hfiles".
     iDestruct (big_sepM_lookup_acc with "Hfiles") as "[HH _]".
     { done. }
-    iSpecialize ("Hlsrv2" $! γlpb with "[]").
-    { iApply "Hlwits". iPureIntro. rewrite /confdγs elem_of_list_In /= //. naive_solver. }
     iModIntro.
     iExists (λ _, True%I), (λ _, True%I), (λ _ _, True%I).
     set (hG' := HeapGS _ _ _).
-    iAssert (file_crash (own_Server_ghost_f γlpb _) []) with "[Hlsrv2]" as "HfileCrash".
-    { iLeft. by iFrame. }
-    iApply (@wpr_kv_replica_main _ _ _ γlpb γsrvl2 with "[$] [$] [$] [$] [$]").
-  }
-  iAssert (is_kv_config dconfigHost γkv) with "[]" as "#Hkvconf".
-  {
-    iDestruct "Hclient_invs2" as (??) "H".
-    repeat iExists _.
-    iDestruct "H" as "( $ & $ & $ )".
-    iFrame "#".
-  }
-  iAssert (is_kv_config lconfigHost γkv0) with "[]" as "#Hlkvconf".
-  {
-    iDestruct "Hlclient_invs2" as (??) "H".
-    repeat iExists _.
-    iDestruct "H" as "( $ & $ & $ )".
-    iFrame "#".
+    iDestruct "Hlsrv" as (?) "[H1 H2]".
+    iApply (wpr_kv_replica_main with "[- $H1]").
+    { iFrame "∗#". }
   }
   iSplitR.
   {
@@ -553,7 +249,8 @@ Proof.
       iApply wp_wpc.
       wp_apply (wp_bank_transferer_main with "[]"); last done.
       repeat iExists _.
-      iFrame "Hbank #".
+      iFrame "Hbank".
+      iSplit. - iExact "Hdhost". - iExact "Hlhost".
     }
     {
       rewrite /hG'.
@@ -563,25 +260,26 @@ Proof.
       iNext.
       simpl.
       set (hG' := HeapGS _ _ hL').
-      iDestruct "Hinvs" as "-#Hinvs".
-      iDestruct "Hkvconf" as "-#Hkvconf".
-      iDestruct "Hlkvconf" as "-#Hlkvconf".
+      iDestruct "Hdhost" as "-#Hdhost".
+      iDestruct "Hlhost" as "-#Hlhost".
       iDestruct "Hbank" as "-#Hbank".
       iCrash.
       iIntros "$".
       destruct hL as [HG'' ?].
-      iDestruct "Hkvconf" as "[%Hheap2 #Hkvconf]"; subst.
-      iDestruct "Hlkvconf" as "[_ #Hlkvconf]".
-      iDestruct "Hbank" as "[_ #Hbank]".
-      clear hG'.
-      clear hL'.
+      set (to_name := (λ x, match x with INamed y => y | _ => "?" end)).
+      repeat iSelect (⌜ _ ⌝ ∗ _)%I
+             (fun H => let x := (eval compute in ("[% " +:+ to_name H +:+ "]")) in
+                    iDestruct H as x).
+      clear hG' hL' HL.
+      subst.
       (* overcome impedence mismatch between heapGS (bundled) and gooseGLobalGS+gooseLocalGS (split) proofs *)
       set (hG2' := HeapGS _ _ goose_localGS).
       simpl.
       iApply wp_wpc.
-      wp_apply (wp_bank_transferer_main with "[]"); last done.
+      wp_apply (wp_bank_transferer_main with "[-]"); last done.
       repeat iExists _.
-      iFrame "Hbank #".
+      iFrame "Hbank".
+      iSplit. - iExact "Hdhost". - iExact "Hlhost".
     }
   }
   iSplitR.
@@ -595,7 +293,8 @@ Proof.
       iApply wp_wpc.
       wp_apply (wp_bank_auditor_main with "[]"); last done.
       repeat iExists _.
-      iFrame "Hbank #".
+      iFrame "Hbank".
+      iSplit. - iExact "Hdhost". - iExact "Hlhost".
     }
     {
       rewrite /hG'.
@@ -605,25 +304,26 @@ Proof.
       iNext.
       simpl.
       set (hG' := HeapGS _ _ hL').
-      iDestruct "Hinvs" as "-#Hinvs".
-      iDestruct "Hkvconf" as "-#Hkvconf".
-      iDestruct "Hlkvconf" as "-#Hlkvconf".
+      iDestruct "Hdhost" as "-#Hdhost".
+      iDestruct "Hlhost" as "-#Hlhost".
       iDestruct "Hbank" as "-#Hbank".
       iCrash.
       iIntros "$".
       destruct hL as [HG'' ?].
-      iDestruct "Hkvconf" as "[%Hheap2 #Hkvconf]"; subst.
-      iDestruct "Hlkvconf" as "[_ #Hlkvconf]".
-      iDestruct "Hbank" as "[_ #Hbank]".
-      clear hG'.
-      clear hL'.
+      set (to_name := (λ x, match x with INamed y => y | _ => "?" end)).
+      repeat iSelect (⌜ _ ⌝ ∗ _)%I
+             (fun H => let x := (eval compute in ("[% " +:+ to_name H +:+ "]")) in
+                    iDestruct H as x).
+      clear hG' hL' HL.
+      subst.
       (* overcome impedence mismatch between heapGS (bundled) and gooseGLobalGS+gooseLocalGS (split) proofs *)
       set (hG2' := HeapGS _ _ goose_localGS).
       simpl.
       iApply wp_wpc.
-      wp_apply (wp_bank_auditor_main with "[]"); last done.
+      wp_apply (wp_bank_auditor_main with "[-]"); last done.
       repeat iExists _.
-      iFrame "Hbank #".
+      iFrame "Hbank".
+      iSplit. - iExact "Hdhost". - iExact "Hlhost".
     }
   }
   done.
